doc/simple/coq/Unif.v
@@ -1,0 +1,574 @@
+Require Import CtxExtension.
+Require Import LibLN.
+Require Import AlgoDef.
+Require Import UtilityEnv.
+Require Import DeclDef.
+Require Import AlgoInfra.
+Require Import DeclInfra.
+Require Import Subst.
+Require Import Theorems.
+Require Import Exists.
+
+Set Implicit Arguments.
+
+Lemma not_in_cpltctx : forall x G H I,
+    ACpltCtxSubstCtx G H I ->
+    x # G ->
+    x # I.
+Proof.
+  intros. inductions H0.
+  auto. apply* IHACpltCtxSubstCtx.
+
+  rewrite dom_push. notin_simpl.
+  rewrite dom_push in H4.
+  auto. apply* IHACpltCtxSubstCtx.
+
+  rewrite dom_push. notin_simpl.
+  rewrite dom_push in H6.
+  auto. apply* IHACpltCtxSubstCtx.
+
+  apply* IHACpltCtxSubstCtx.
+  apply* IHACpltCtxSubstCtx.
+  apply* IHACpltCtxSubstCtx.
+Qed.
+
+Lemma ctxsubst_comm_app : forall G e1 e2,
+    ACtxSubst G (AE_App e1 e2) = AE_App (ACtxSubst G e1) (ACtxSubst G e2).
+Proof.
+  intros. gen e1 e2. induction G using env_ind; intros.
+  rewrite subst_empty_env.
+  rewrite subst_empty_env.
+  rewrite subst_empty_env.
+  auto.
+  inductions v.
+  rewrite subst_add_var.
+  rewrite subst_add_var.
+  rewrite subst_add_var.
+  auto.
+  rewrite subst_add_typvar.
+  rewrite subst_add_typvar.
+  rewrite subst_add_typvar.
+  auto.
+  rewrite subst_add_bndvar.
+  rewrite subst_add_bndvar.
+  rewrite subst_add_bndvar.
+  apply* IHG.
+  rewrite subst_add_evar.
+  rewrite subst_add_evar.
+  rewrite subst_add_evar.
+  auto.
+  rewrite subst_add_solved_evar.
+  rewrite subst_add_solved_evar.
+  rewrite subst_add_solved_evar.
+  apply* IHG.
+Qed.
+
+Lemma ctxsubst_id_app: forall G e1 e2,
+    AE_App e1 e2 = ACtxSubst G (AE_App e1 e2) ->
+    e1 = ACtxSubst G e1.
+Proof.
+  intros. induction G using env_ind.
+  rewrite subst_empty_env. auto.
+  inductions v.
+  rewrite subst_add_var in H.
+  rewrite subst_add_var. apply* IHG.
+  rewrite subst_add_typvar in H.
+  rewrite subst_add_typvar. apply* IHG.
+  rewrite subst_add_bndvar in H.
+  simpl in H.
+  rewrite subst_add_bndvar.
+  rewrite ctxsubst_comm_app in H.
+  injection H; intros. auto.
+  rewrite subst_add_evar.
+  rewrite subst_add_evar in H.
+  apply* IHG.
+  rewrite subst_add_solved_evar in H.
+  simpl in H.
+  rewrite ctxsubst_comm_app in H.
+  injection H; intros.
+  rewrite subst_add_solved_evar.
+  auto.
+Qed.
+
+Lemma ctxsubst_comm_ann : forall G e1 e2,
+    ACtxSubst G (AE_Ann e1 e2) = AE_Ann (ACtxSubst G e1) (ACtxSubst G e2).
+Proof.
+  intros. gen e1 e2. induction G using env_ind; intros.
+  rewrite subst_empty_env.
+  rewrite subst_empty_env.
+  rewrite subst_empty_env.
+  auto.
+  inductions v.
+  rewrite subst_add_var.
+  rewrite subst_add_var.
+  rewrite subst_add_var.
+  auto.
+  rewrite subst_add_typvar.
+  rewrite subst_add_typvar.
+  rewrite subst_add_typvar.
+  auto.
+  rewrite subst_add_bndvar.
+  rewrite subst_add_bndvar.
+  rewrite subst_add_bndvar.
+  apply* IHG.
+  rewrite subst_add_evar.
+  rewrite subst_add_evar.
+  rewrite subst_add_evar.
+  auto.
+  rewrite subst_add_solved_evar.
+  rewrite subst_add_solved_evar.
+  rewrite subst_add_solved_evar.
+  apply* IHG.
+Qed.
+
+Lemma ctxsubst_id_ann: forall G e1 e2,
+    AE_Ann e1 e2 = ACtxSubst G (AE_Ann e1 e2) ->
+    e1 = ACtxSubst G e1.
+Proof.
+  intros. induction G using env_ind.
+  rewrite subst_empty_env. auto.
+  inductions v.
+  rewrite subst_add_var in H.
+  rewrite subst_add_var. apply* IHG.
+  rewrite subst_add_typvar in H.
+  rewrite subst_add_typvar. apply* IHG.
+  rewrite subst_add_bndvar in H.
+  simpl in H.
+  rewrite subst_add_bndvar.
+  rewrite ctxsubst_comm_ann in H.
+  injection H; intros. auto.
+  rewrite subst_add_evar.
+  rewrite subst_add_evar in H.
+  apply* IHG.
+  rewrite subst_add_solved_evar in H.
+  simpl in H.
+  rewrite ctxsubst_comm_ann in H.
+  injection H; intros.
+  rewrite subst_add_solved_evar.
+  auto.
+Qed.
+
+Lemma ctxsubst_comm_castup : forall G e1,
+    ACtxSubst G (AE_CastUp e1) = AE_CastUp (ACtxSubst G e1).
+Proof.
+  intros. gen e1. induction G using env_ind; intros.
+  rewrite subst_empty_env.
+  rewrite subst_empty_env.
+  auto.
+  inductions v.
+  rewrite subst_add_var.
+  rewrite subst_add_var.
+  auto.
+  rewrite subst_add_typvar.
+  rewrite subst_add_typvar.
+  auto.
+  rewrite subst_add_bndvar.
+  rewrite subst_add_bndvar.
+  apply* IHG.
+  rewrite subst_add_evar.
+  rewrite subst_add_evar.
+  auto.
+  rewrite subst_add_solved_evar.
+  rewrite subst_add_solved_evar.
+  apply* IHG.
+Qed.
+
+Lemma ctxsubst_id_castup: forall G e1,
+    AE_CastUp e1 = ACtxSubst G (AE_CastUp e1) ->
+    e1 = ACtxSubst G e1.
+Proof.
+  intros. induction G using env_ind.
+  rewrite subst_empty_env. auto.
+  inductions v.
+  rewrite subst_add_var in H.
+  rewrite subst_add_var. apply* IHG.
+  rewrite subst_add_typvar in H.
+  rewrite subst_add_typvar. apply* IHG.
+  rewrite subst_add_bndvar in H.
+  simpl in H.
+  rewrite subst_add_bndvar.
+  rewrite ctxsubst_comm_castup in H.
+  injection H; intros. auto.
+  rewrite subst_add_evar.
+  rewrite subst_add_evar in H.
+  apply* IHG.
+  rewrite subst_add_solved_evar in H.
+  simpl in H.
+  rewrite ctxsubst_comm_castup in H.
+  injection H; intros.
+  rewrite subst_add_solved_evar.
+  auto.
+Qed.
+
+Lemma ctxsubst_comm_castdn : forall G e1,
+    ACtxSubst G (AE_CastDn e1) = AE_CastDn (ACtxSubst G e1).
+Proof.
+  intros. gen e1. induction G using env_ind; intros.
+  rewrite subst_empty_env.
+  rewrite subst_empty_env.
+  auto.
+  inductions v.
+  rewrite subst_add_var.
+  rewrite subst_add_var.
+  auto.
+  rewrite subst_add_typvar.
+  rewrite subst_add_typvar.
+  auto.
+  rewrite subst_add_bndvar.
+  rewrite subst_add_bndvar.
+  apply* IHG.
+  rewrite subst_add_evar.
+  rewrite subst_add_evar.
+  auto.
+  rewrite subst_add_solved_evar.
+  rewrite subst_add_solved_evar.
+  apply* IHG.
+Qed.
+
+Lemma ctxsubst_id_castdn: forall G e1,
+    AE_CastDn e1 = ACtxSubst G (AE_CastDn e1) ->
+    e1 = ACtxSubst G e1.
+Proof.
+  intros. induction G using env_ind.
+  rewrite subst_empty_env. auto.
+  inductions v.
+  rewrite subst_add_var in H.
+  rewrite subst_add_var. apply* IHG.
+  rewrite subst_add_typvar in H.
+  rewrite subst_add_typvar. apply* IHG.
+  rewrite subst_add_bndvar in H.
+  simpl in H.
+  rewrite subst_add_bndvar.
+  rewrite ctxsubst_comm_castdn in H.
+  injection H; intros. auto.
+  rewrite subst_add_evar.
+  rewrite subst_add_evar in H.
+  apply* IHG.
+  rewrite subst_add_solved_evar in H.
+  simpl in H.
+  rewrite ctxsubst_comm_castdn in H.
+  injection H; intros.
+  rewrite subst_add_solved_evar.
+  auto.
+Qed.
+
+Lemma awtyp_expr_wf: forall G a,
+    AWfTyp G (AT_Expr a) ->
+    AWTerm G a.
+Proof.
+  intros. inductions H; intros.
+  apply* AWTerm_EVar.
+  apply* AWTerm_Solved_EVar.
+  apply AWTerm_Pi with (L:=L). auto.
+  intros. rewrite <- (concat_empty_r (G & x ~ AC_Var)).
+  apply awterm_replace with (t := t1).
+  rewrite -> (concat_empty_r (G & x ~ AC_Typ t1)).
+  apply* H1.
+  apply* atyping_awterm.
+Qed.
+
+Lemma awterm_typ: forall G x a,
+    AWf (G & x ~ AC_Typ a) ->
+    AWTerm G a.
+Proof.
+  intros. inductions H.
+  false. apply* empty_push_inv.
+  destruct (eq_push_inv x) as [? [? ?]]. inversions H2.
+  destruct (eq_push_inv x) as [? [? ?]]. inversions H3.
+  inversions H1. apply* AWTerm_EVar. apply* AWTerm_Solved_EVar.
+  apply AWTerm_Pi with (L:=L). apply* awtyp_expr_wf.
+  intros. rewrite <- (concat_empty_r (G & x0 ~ AC_Var)).
+  apply awterm_replace with (t := t1).
+  rewrite -> (concat_empty_r (G & x0 ~ AC_Typ t1)).
+  pose (H5 x0 H1).
+  apply* awtyp_expr_wf.
+  apply* atyping_awterm.
+  destruct (eq_push_inv x) as [? [? ?]]. inversions H5.
+  destruct (eq_push_inv x) as [? [? ?]]. inversions H5.
+  destruct (eq_push_inv x) as [? [? ?]]. inversions H2.
+  destruct (eq_push_inv x) as [? [? ?]]. inversions H3.
+Qed.
+
+Lemma awtermt_bnd: forall G x s t,
+    AWf (G & x ~ AC_Bnd s t) ->
+    AWTermT G s.
+Proof.
+  introv wf. gen_eq H : (G & x ~ AC_Bnd s t).
+  gen G s. induction wf; introv hi; try(
+  solve[apply eq_push_inv in hi; destruct hi as [eqx [eqv eqg]]; inversion eqv]); subst; auto.
+  apply empty_push_inv in hi. inversion hi.
+  apply eq_push_inv in hi; destruct hi as [eqx [eqv eqg]]; inversion eqv. subst. apply* AWTermT_Expr. apply* awtyp_expr_wf.
+
+  apply eq_push_inv in hi; destruct hi as [eqx [eqv eqg]]. inversion eqv. subst.
+  apply AWTermT_Forall with (L := L). intros.
+  apply (H2 x0 H3). auto.
+Qed.
+
+Theorem cpltctxsubstctx_exists: forall G,
+    AWf G ->
+    CompleteCtx G ->
+    exists H, ACpltCtxSubstCtx G G H.
+Proof.
+  intros.
+  induction G using env_ind.
+  exists* (empty : DCtx). apply* ACpltCtxSubstCtx_Empty.
+  assert (WfG : AWf G) by (apply* AWf_left).
+  assert (CCtxG : CompleteCtx G) by (apply* complete_part_left; apply* awf_is_ok).
+  induction v.
+
+  destruct (IHG WfG CCtxG) as [H1 IHSubst].
+  exists H1. apply* ACpltCtxSubstCtx_Var.
+
+  assert (TrmA: AWTerm G a) by (apply* awterm_typ).
+  destruct (cpltctxsubst_exists G a WfG TrmA CCtxG) as [t1' S].
+  destruct (IHG WfG CCtxG) as [H1 S'].
+  exists (H1 & x ~ DC_Typ t1'). apply* ACpltCtxSubstCtx_TypVar.
+
+  assert (TrmA: AWTerm G a0) by (apply* awterm_bnd).
+  destruct (cpltctxsubst_exists G a0 WfG TrmA CCtxG) as [t1' S].
+  destruct (IHG WfG CCtxG) as [H1 S'].
+  assert (TrmAT: AWTermT G a) by (apply* awtermt_bnd).
+  destruct (cpltctxtsubst_exists G a WfG TrmAT CCtxG) as [t2' S2].
+  exists (H1 & x ~ DC_Bnd t2' t1'). apply* ACpltCtxSubstCtx_BndVar.
+
+  false. unfold CompleteCtx in H0.
+  destruct (H0 x AC_Unsolved_EVar).
+  apply* binds_tail. auto.
+
+  destruct (IHG WfG CCtxG) as [H1 IHSubst].
+  exists H1. apply* ACpltCtxSubstCtx_Solved_Solved_EVar.
+Qed.
+
+Lemma confluence_cplt2 : forall G1 G2 H I J,
+    ExtCtx G1 H -> ExtCtx G2 H ->
+    CompleteCtx H ->
+    ACpltCtxSubstCtx H G1 I ->
+    ACpltCtxSubstCtx H G2 J ->
+    I = J.
+Proof.
+  intros.
+  assert (Wf: AWf H) by (apply* awf_preservation).
+  destruct (cpltctxsubstctx_exists Wf H2) as [K P].
+  assert (I = K).
+  intros. apply stable_cplt_env_eq with (G := G1) (H := H).
+  auto. auto. auto.
+  assert (J = K).
+  intros. apply stable_cplt_env_eq with (G := G2) (H := H).
+  auto. auto. auto.
+  subst. auto.
+Qed.
+
+Lemma extctx_remove_var : forall G H y,
+    ExtCtx (G & y ~ AC_Var) (H & y ~ AC_Var) ->
+    ExtCtx G H.
+Proof.
+  introv D.
+  rewrite <- concat_empty_r in D at 1.
+  rewrite <- concat_empty_r in D.
+  destruct (extension_order_var D) as [X [Y (K1 & K2 & _)]].
+  lets C: awf_preservation D.
+  pose (Ok2 := awf_is_ok C).
+  lets Ok3: Ok2.
+  rewrite K1 in Ok3.
+  destruct~ (ok_middle_eq Ok2 eq_refl Ok3 eq_refl K1) as (Eq1 & Eq2 & Eq3).
+  subst*.
+Qed.
+
+Lemma extctx_remove_typvar : forall G H y t1 t2,
+    ExtCtx (G & y ~ AC_Typ t1) (H & y ~ AC_Typ t2) ->
+    ExtCtx G H.
+Proof.
+  introv D.
+  rewrite <- concat_empty_r in D at 1.
+  rewrite <- concat_empty_r in D.
+  destruct (extension_order_typvar D) as [X [Y [Z (K1 & K2 & _)]]].
+  lets C: awf_preservation D.
+  pose (Ok2 := awf_is_ok C).
+  lets Ok3: Ok2.
+  rewrite K1 in Ok3.
+  destruct~ (ok_middle_eq Ok2 eq_refl Ok3 eq_refl K1) as (Eq1 & Eq2 & Eq3).
+  subst*.
+Qed.
+
+Lemma extctx_remove_exists : forall G I y v,
+    ExtCtx G (I & y ~ v) ->
+    exists G', G = G' & y ~ v /\ ExtCtx G' I.
+Admitted.
+
+Lemma extctx_to_empty_inv : forall G,
+    ExtCtx G empty -> G = empty.
+Proof.
+  intros.
+  inversions H; auto; false; apply* empty_push_inv.
+Qed.
+
+Theorem cpltctxsubstctx_exists_ext: forall G I,
+    ExtCtx I G ->
+    CompleteCtx G ->
+    exists H, ACpltCtxSubstCtx G I H.
+Proof.
+  intros. gen I.
+  induction G using env_ind; intros.
+  assert (I = empty) by (apply* extctx_to_empty_inv).
+  subst.
+  exists* (empty : DCtx). apply* ACpltCtxSubstCtx_Empty.
+  lets:  awf_preservation H.
+  destruct (extctx_remove_exists H) as [I' [Eq Ext']].
+  assert (WfG : AWf G) by (apply* AWf_left).
+  assert (CCtxG : CompleteCtx G) by (apply* complete_part_left; apply* awf_is_ok).
+  induction v.
+  
+  destruct (IHG CCtxG I' Ext') as [H1' IHSubst].
+  exists H1'. rewrite Eq. apply* ACpltCtxSubstCtx_Var.
+
+  assert (TrmA: AWTerm G a) by (apply* awterm_typ).
+  destruct (cpltctxsubst_exists G a WfG TrmA CCtxG) as [t1' S].
+  destruct (IHG CCtxG I' Ext') as [H1' S'].
+  exists (H1' & x ~ DC_Typ t1'). rewrite Eq. apply* ACpltCtxSubstCtx_TypVar.
+
+  assert (TrmA: AWTerm G a0) by (apply* awterm_bnd).
+  destruct (cpltctxsubst_exists G a0 WfG TrmA CCtxG) as [t1' S].
+  destruct (IHG CCtxG I' Ext') as [H1' S'].
+  assert (TrmAT: AWTermT G a) by (apply* awtermt_bnd).
+  destruct (cpltctxtsubst_exists G a WfG TrmAT CCtxG) as [t2' S2].
+  exists (H1' & x ~ DC_Bnd t2' t1'). rewrite Eq. apply* ACpltCtxSubstCtx_BndVar.
+
+  false. unfold CompleteCtx in H0.
+  destruct (H0 x AC_Unsolved_EVar).
+  apply* binds_tail. auto.
+
+  destruct (IHG CCtxG I' Ext') as [H1' IHSubst].
+  exists H1'. rewrite Eq. apply* ACpltCtxSubstCtx_Solved_Solved_EVar.
+Qed.
+
+Lemma confluence_cplt3 : forall G1 G2 H I,
+    ExtCtx G1 H -> ExtCtx G2 H ->
+    CompleteCtx H ->
+    ACpltCtxSubstCtx H G1 I ->
+    ACpltCtxSubstCtx H G2 I.
+Proof.
+  intros.
+  destruct (cpltctxsubstctx_exists_ext H1 H2) as [J ?].
+  assert (I = J).
+  apply (confluence_cplt2 H0 H1 H2 H3 H4).
+  subst. auto.
+Qed.
+
+Lemma unif_to_extctx : forall G H t1 t2,
+    AWf G ->
+    AUnify G t1 t2 H ->
+    AWf H /\ ExtCtx G H.
+Proof.
+  intros. inductions H1; try solve [split*; apply* extension_reflexivity].
+
+  destruct (IHAUnify1 H0) as [A B].
+  destruct (IHAUnify2 A) as [A1 B1].
+  split*. apply* extension_transitivity.
+
+  destruct (IHAUnify H0) as [A B].
+  pick_fresh_gen (L \u dom H1) y.
+  assert (y \notin L) by auto.
+  destruct (H4 y H5) as [C D].
+  apply AWf_Var. auto. auto.
+  split. apply* AWf_left. apply* extension_transitivity.
+  apply* extctx_remove_var.
+
+  pick_fresh_gen (L \u dom G) y.
+  assert (y \notin L) by auto.
+  destruct (H2 y H3) as [C D].
+  apply AWf_Var. auto. auto.
+  split. apply* AWf_left. 
+  apply* extctx_remove_var.
+
+  destruct (IHAUnify H0) as [A B].
+  pick_fresh_gen (L \u dom H1) y.
+  assert (y \notin L) by auto.
+  destruct (H4 y H5) as [C D].
+  apply AWf_TyVar. auto. auto. admit.
+  split. apply* AWf_left. apply* extension_transitivity.
+  apply* extctx_remove_typvar.
+  
+  destruct (IHAUnify1 H0) as [A B].
+  destruct (IHAUnify2 A) as [A1 B1].
+  split*. apply* extension_transitivity.
+
+  admit. admit.
+Qed.
+
+Theorem unif_soundness : forall G H I t1 t2 H' t1' t2',
+    AUnify G t1 t2 H ->
+    t1 = ACtxSubst G t1 ->
+    t2 = ACtxSubst G t2 ->
+    ExtCtx H I ->
+    CompleteCtx I ->
+    ACpltCtxSubstCtx I H H' ->
+    ACpltCtxSubst I t1 t1' ->
+    ACpltCtxSubst I t2 t2' ->
+    AWf G ->
+    t1' = t2'.
+Proof.
+  intros. gen t1'. gen t2'. inductions H0; intros.
+
+  apply* cplt_ctxsubst_eq.
+  apply* cplt_ctxsubst_eq.
+  apply* cplt_ctxsubst_eq.
+  apply* cplt_ctxsubst_eq.
+  
+  inversions H6. inversions H7.
+  auto.
+
+  inversions H6. inversions H7.
+  destruct (unif_to_extctx H8 H0_) as [Wf _].
+  destruct (unif_to_extctx Wf H0_0) as [_ Ext].
+  pose (ctxsubst_id_app G H0).
+  pose (ctxsubst_id_app G H2).
+  assert (d1 = d0).
+  apply* IHAUnify1. 
+  apply* extension_transitivity.
+  apply* confluence_cplt3.
+  apply* extension_transitivity.
+  assert (d2 = d3).
+  apply* cplt_ctxsubst_eq.
+  rewrite H6. rewrite H7. auto.
+
+  inversions H11. inversions H10. admit.
+
+  inversions H7. inversions H9. admit.
+
+  inversions H6. inversions H7.
+  destruct (unif_to_extctx H8 H0) as [Wf Ext].
+  pose (ctxsubst_id_castup G H1).
+  pose (ctxsubst_id_castup G H2).
+  assert (d = d0).
+  apply* IHAUnify. 
+  rewrite H6. auto.
+
+  inversions H6. inversions H7.
+  destruct (unif_to_extctx H8 H0) as [Wf Ext].
+  pose (ctxsubst_id_castdn G H1).
+  pose (ctxsubst_id_castdn G H2).
+  assert (d = d0).
+  apply* IHAUnify. 
+  rewrite H6. auto.
+
+  inversions H10. inversions H11. admit.
+
+  inversions H6. inversions H7.
+  destruct (unif_to_extctx H8 H0_) as [Wf _].
+  destruct (unif_to_extctx Wf H0_0) as [_ Ext].
+  pose (ctxsubst_id_ann G H0).
+  pose (ctxsubst_id_ann G H2).
+  assert (d1 = d0).
+  apply* IHAUnify1. 
+  apply* extension_transitivity.
+  apply* confluence_cplt3.
+  apply* extension_transitivity.
+  assert (d2 = d3).
+  apply* cplt_ctxsubst_eq.
+  rewrite H6. rewrite H7. auto.
+
+  admit.
+
+  admit.
+Qed.
+
